theories/Semantics.v
@@ -4,7 +4,7 @@ From MetaCoq.Erasure.Typed Require Import Annotations.
 From MetaCoq.Erasure Require Import EAst ECSubst ELiftSubst EWellformed.
 From MetaCoq.Utils Require Import utils.
 
-From VTL Require Import PIR BigStepPIR Subset Translation Utils.
+From VTL Require Import Entry PIR BigStepPIR Subset Translation Utils.
 
 Existing Instance EWcbvEval.default_wcbv_flags.
 Set Default Goal Selector "!".
@@ -16,65 +16,144 @@ Import MCMonadNotation.
 Definition gal_id :=
   tLambda (BasicAst.nNamed "x"%bs) (tRel 0).
 
-Lemma lookup_entry_Some : forall Σ_fresh kn kn' br, 
-  lookup_entry Σ_fresh kn = Some (kn, kn', br) ->
-  In kn' (map (snd ∘ fst) Σ_fresh).
-Proof.
-  intros. induction Σ_fresh.
-  - discriminate.
-  - destruct a as [[bd_kn bd_kn'] bd]. 
-    simpl. simpl in H.
-    destruct (bd_kn == kn) eqn:Heq; inversion H; subst.
-    + now left.
-    + apply IHΣ_fresh in H1. now right.
-Qed.
-
-Lemma lookup_fresh_Some : forall Σ_fresh kn kn', 
-  lookup_fresh Σ_fresh kn = Some (kn, kn') ->
-  In kn' (map snd Σ_fresh).
-Proof.
-  intros. induction Σ_fresh.
-  - discriminate.
-  - destruct a as [bd_kn bd_kn']. 
-    simpl. simpl in H. eauto.
-    destruct (bd_kn == kn) eqn:Heq; inversion H; subst.
-    + now left.
-    + apply IHΣ_fresh in H1. now right.
-Qed.
-
-Lemma lookup_init : forall Σ Σ' ann_env kn kn' decl cb,
-  EGlobalEnv.declared_constant (trans_env Σ) kn decl ->
+Lemma lookup_init : forall eΣ Σ' ann_env kn kn' decl cb,
+  EGlobalEnv.declared_constant (trans_env eΣ) kn decl ->
   decl.(EAst.cst_body) = Some cb ->
-  lookup_fresh (map fst Σ') kn = Some (kn, kn') ->
-  translatesEnv remap_env Σ Σ' ann_env ->
+  lookup_fresh (to_fresh_map Σ') kn = Some (kn, kn') ->
+  translatesEnv remap_env eΣ Σ' ann_env ->
   exists Σ'' ann_cb cb', translatesTo remap_env Σ'' [] cb ann_cb cb'.
 Proof.
-  intros. induction Σ.
+  intros. induction H2.
   - discriminate.
-  - destruct a as [[c_kn c_kn'] c_decl].
-    hnf in H. simpl in H.
-    destruct (kn == c_kn).
-    + destruct c_decl.
-      * inversion H2. subst.
-        destruct entry as [[e_kn e_kn'] [vd b]].
-        destruct c. destruct cst_body; simpl in H9; try eauto.
-        destruct decl. destruct cst_body; try discriminate.
-        inversion H. inversion H0. subst. hnf in ann_decl.
-        exists (map fst Σ'0). exists ann_decl. exists b. 
-        assumption.
+  - destruct entry as [e_kn [[e_kn' ty'] e_b']].
+    hnf in H. simpl in H, H1.
+    destruct (kn == kn0) eqn:Heq.
+    + destruct decl0.
+      * destruct c. destruct cst_body; simpl in H2; try eauto.
+        destruct decl; try discriminate.
+        destruct cst_body; try discriminate. 
+        inversion H. invs H0.
+        exists (to_fresh_map Σ'). exists ann_decl. exists e_b'.
+        assumption. 
       * inversion H.
-      * inversion H. inversion H2. subst.
-        admit.
-    + inversion H2.
       * admit.
-      * eapply IHΣ; try eauto.
+    + eapply IHtranslatesEnv; try eauto.
+      simpl in H1. destruct (e_kn == kn); try eauto.
+      invs H1. admit.
 Admitted.
 
-Lemma weaken_ctx : forall Σ_fresh Γ x t ann t',
-  translatesTo remap_env Σ_fresh Γ t ann t' ->
-  translatesTo remap_env Σ_fresh (Γ ++ [x]) t ann t'.
+Fixpoint subst_entries (Σ' : list entry) t {struct Σ'} :=
+  match Σ' with
+  | [] => t
+  | ((_, TermBind (VarDecl kn' ty) b)::Σ'') => 
+      BigStepPIR.subst kn' b (subst_entries Σ'' t)
+  end.
+
+Fixpoint subst_bnr_entries (Σ' : list entry) bnd {struct Σ'} :=
+  match Σ' with
+  | [] => bnd
+  | ((_, TermBind (VarDecl kn' ty) b)::Σ'') => 
+      @subst_bnr' subst_b kn' b (subst_bnr_entries Σ'' bnd)
+  end.
+
+Lemma unfold_app_subst x v' f' a' :
+  BigStepPIR.subst x v' (Apply f' a') = Apply (BigStepPIR.subst x v' f') (BigStepPIR.subst x v' a').
 Proof.
-  intros Σ_fresh Γ x t. revert Γ.
+  eauto.
+Qed.
+
+Lemma unfold_app_subst_entries (Σ' : list entry) f' a' :
+  subst_entries Σ' (Apply f' a') = Apply (subst_entries Σ' f') (subst_entries Σ' a').
+Proof.
+  induction Σ'.
+  - eauto.
+  - destruct a as [fr [[] b]].
+    simpl. now rewrite <- unfold_app_subst.
+Qed.
+
+Lemma unfold_let_subst x v' bs t' :
+  BigStepPIR.subst x v' (Let bs t') =
+  Let (@subst_bnr' subst_b x v' bs)
+      (if existsb (eqb x) (bvbs bs)
+        then t'
+        else BigStepPIR.subst x v' t').
+Proof.
+  eauto.
+Qed.
+
+Lemma unfold_let_subst_entries Σ' e_kn e_kn' e_ty e_b' bs t' :
+  subst_entries ((e_kn, TermBind (VarDecl e_kn' e_ty) e_b') :: Σ')
+    (Let bs t')
+  =
+  Let
+    (@subst_bnr' subst_b e_kn' e_b' (subst_bnr_entries Σ' bs))
+    (if existsb (eqb e_kn') (bvbs bs)
+     then t'
+     else (BigStepPIR.subst e_kn' e_b' (subst_entries Σ' t'))).
+Proof.
+  induction Σ'.
+  - eauto.
+  - destruct a as [a_kn [[nm ty] t]]. simpl in *.
+    admit.
+Admitted. 
+
+Lemma subst_not_free : forall x v b,
+  ~ In x (fv b) ->
+  subst x v b = b.
+Proof.
+Admitted.
+
+Lemma subst_comm : forall x y n l m,
+  x <> y ->
+  ~ In x (fv l) ->
+  BigStepPIR.subst x n (BigStepPIR.subst y l m) = 
+  BigStepPIR.subst y l (BigStepPIR.subst x n m).
+Proof.
+  intros. induction m; try eauto.
+  - admit.
+  - admit.
+  - destruct_str_eq y b.
+    + simpl. rewrite Heqb.
+      destruct_str_eq x b.
+      * subst. contradiction.
+      * simpl. now rewrite Heqb, Heqb0.
+    + simpl. rewrite Heqb.
+      destruct_str_eq x b.
+      * simpl. now rewrite Heqb, Heqb0.
+      * simpl. now rewrite Heqb, Heqb0, IHm.
+  - simpl. f_equal; eauto.
+Admitted.
+
+Lemma subst_entries_comm : forall (Σ' : list entry) x v b,
+  ~ In x (map get_entry_nm Σ') ->
+  BigStepPIR.subst x v (subst_entries Σ' b) = subst_entries Σ' (BigStepPIR.subst x v b).
+Proof.
+  intros. induction Σ'.
+  - eauto.
+  - destruct a as [[e_kn e_kn'] [[nm ty] t]].
+    simpl in *. rewrite subst_comm.
+    + f_equal. now apply IHΣ'.
+    + now apply not_in_cons in H as [Hneq HnIn].
+    + apply not_in_cons in H. admit.
+Admitted.
+
+Lemma eval_constant_unfolding : forall Σ' kn' b' v' k,
+  ~ In kn' (map get_entry_nm Σ') ->
+  eval (subst_entries Σ' b') v' k ->
+  eval (subst kn' b' (subst_entries Σ' (Var kn'))) v' k.
+Proof.
+  intros. revert b' H0. induction Σ'; intros.
+  - simpl. intros. now rewrite eqb_refl.
+  - destruct a as [e_kn [[nm ty] t]].
+    rewrite subst_entries_comm; try eauto.
+    simpl. now rewrite eqb_refl.
+Qed.
+
+Lemma weaken_ctx : forall frmap Γ x t ann t',
+  translatesTo remap_env frmap Γ t ann t' ->
+  translatesTo remap_env frmap (Γ ++ [x]) t ann t'.
+Proof.
+  intros frmap Γ x t. revert Γ.
   induction t; intros Γ ann t' tlt;
   inversion tlt; subst.
   - constructor.
@@ -95,11 +174,11 @@ Proof.
   - now eapply tlt_const.
 Qed.
 
-Lemma weaken_ctx_many : forall Σ_fresh Γ1 Γ2 t ann t',
-  translatesTo remap_env Σ_fresh Γ1 t ann t' ->
-  translatesTo remap_env Σ_fresh (Γ1 ++ Γ2) t ann t'.
+Lemma weaken_ctx_many : forall frmap Γ1 Γ2 t ann t',
+  translatesTo remap_env frmap Γ1 t ann t' ->
+  translatesTo remap_env frmap (Γ1 ++ Γ2) t ann t'.
 Proof.
-  intros Σ_fresh Γ1 Γ2 t. revert Γ1. induction t;
+  intros frmap Γ1 Γ2 t. revert Γ1. induction t;
   intros Γ1 ann t' tlt_t; 
   inversion tlt_t; subst.
   - constructor.
@@ -120,12 +199,12 @@ Proof.
   - now eapply tlt_const.
 Qed.
 
-Lemma strengthen_shadowed_ctx : forall Σ_fresh Γ x b ann_b b',
+Lemma strengthen_shadowed_ctx : forall frmap Γ x b ann_b b',
   In x Γ ->
-  translatesTo remap_env Σ_fresh (Γ ++ [x]) b ann_b b' ->
-  translatesTo remap_env Σ_fresh Γ b ann_b b'.
+  translatesTo remap_env frmap (Γ ++ [x]) b ann_b b' ->
+  translatesTo remap_env frmap Γ b ann_b b'.
 Proof.
-  intros Σ_fresh Γ x b. revert Γ. induction b;
+  intros frmap Γ x b. revert Γ. induction b;
   intros Γ ann_b b' Hin tlt; inversion tlt; subst.
   - constructor.
   - apply tlt_rel.
@@ -181,122 +260,13 @@ Proof.
     exact (f _ _ X).
 Defined.
 
-Fixpoint subst_entries (Σ' : list entry) t {struct Σ'} :=
-  match Σ' with
-  | [] => t
-  | ((_, TermBind (VarDecl kn' ty) b)::Σ'') => 
-      BigStepPIR.subst kn' b (subst_entries Σ'' t)
-  end.
-
-Lemma unfold_app_subst x v' f' a' :
-  BigStepPIR.subst x v' (Apply f' a') = Apply (BigStepPIR.subst x v' f') (BigStepPIR.subst x v' a').
-Proof.
-  eauto.
-Qed.
-
-Lemma unfold_app_subst_entries (Σ' : list entry) f' a' :
-  subst_entries Σ' (Apply f' a') = Apply (subst_entries Σ' f') (subst_entries Σ' a').
-Proof.
-  induction Σ'.
-  - eauto.
-  - destruct a as [fr [[] b]].
-    simpl. now rewrite <- unfold_app_subst.
-Qed.
-
-Lemma unfold_let_subst x v' bs t' :
-  BigStepPIR.subst x v' (Let bs t') =
-  Let (@subst_bnr' subst_b x v' bs)
-      (if existsb (eqb x) (bvbs bs)
-        then t'
-        else BigStepPIR.subst x v' t').
-Proof.
-  eauto.
-Qed.
-
-Lemma subst_comm : forall kn kn' v v' b,
-  kn <> kn' ->
-  BigStepPIR.subst kn v (BigStepPIR.subst kn' v' b) = BigStepPIR.subst kn' v' (BigStepPIR.subst kn v b).
-Proof.
-  intros. induction b; try eauto.
-  - admit.
-  - admit.
-  - destruct_str_eq kn' b.
-    + simpl. rewrite Heqb.
-      destruct_str_eq kn b.
-      * subst. contradiction.
-      * simpl. now rewrite Heqb, Heqb0.
-    + simpl. rewrite Heqb.
-      destruct_str_eq kn b.
-      * simpl. now rewrite Heqb, Heqb0.
-      * simpl. now rewrite Heqb, Heqb0, IHb.
-  - simpl. f_equal; eauto.
-Admitted.
-
-Lemma subst_entries_comm : forall (Σ' : list entry) x v b,
-  ~ In x (map (fun '((_, _), TermBind (VarDecl nm _) _) => nm) Σ') ->
-  BigStepPIR.subst x v (subst_entries Σ' b) = subst_entries Σ' (BigStepPIR.subst x v b).
-Proof.
-  intros. induction Σ'.
-  - eauto.
-  - destruct a as [[e_kn e_kn'] [[nm ty] t]].
-    simpl in *. rewrite subst_comm.
-    + now rewrite IHΣ'.
-    + now apply not_in_cons in H as [Hneq HnIn].
-Qed.
-
-Lemma unfold_let_subst_entries Σ' e_kn e_kn' e_ty e_b' bs t' :
-  subst_entries (((e_kn, e_kn'), TermBind (VarDecl e_kn' e_ty) e_b') :: Σ')
-    (Let bs t')
-  =
-  Let
-    (@subst_bnr' subst_b e_kn' e_b' bs)
-    (if existsb (eqb e_kn') (bvbs bs)
-     then t'
-     else (BigStepPIR.subst e_kn' e_b' (subst_entries Σ' t'))).
-Proof.
-  induction Σ'.
-  - eauto.
-  - destruct a as [[a_kn a_kn'] [[nm ty] t]]. simpl in *.
-    admit.
-Admitted. 
-
-Lemma eval_constant_unfolding : forall Σ' kn' b' v' k,
-  (forall e : entry, match e with | ((_, e_kn'), TermBind (VarDecl e_nm _) _) => e_kn' = e_nm end) ->  
-  ~ In kn' (map (fun '((_, _), TermBind (VarDecl nm _) _) => nm) Σ') ->
-  eval (subst_entries Σ' b') v' k ->
-  eval (subst kn' b' (subst_entries Σ' (Var kn'))) v' k.
-Proof.
-  intros. revert b' H1. induction Σ'; intros.
-  - simpl. intros. now rewrite eqb_refl.
-  - destruct a as [[e_kn e_kn'] [[nm ty] t]].
-    rewrite subst_entries_comm; try eauto.
-    simpl. now rewrite eqb_refl.
-Qed.
-
-Lemma eval_value : forall Σ' v' k,
-  eval v' v' k ->
-  exists j, eval (subst_entries Σ' v') v' j.
-Proof.
-  intros Σ' v' k ev. 
-  induction Σ'; eauto.
-  destruct a as [[e_kn e_kn'] [[nm ty] t]].
-  inversion ev; subst.
-  - simpl. rewrite subst_entries_comm; [|admit].
-    simpl. destruct_str_eq nm x.
-    + apply IHΣ'.
-    + admit.
-  - admit.
-  - simpl. now rewrite subst_entries_comm; [|admit].
-  - admit.
-Admitted.
-
-Lemma csubst_shadowed : forall Σ_fresh Γ x b ann_b b' v ann_v,
+Lemma csubst_shadowed : forall frmap Γ x b ann_b b' v ann_v,
   In x Γ ->
-  translatesTo remap_env Σ_fresh (Γ ++ [x]) b ann_b b' ->
-  translatesTo remap_env Σ_fresh (Γ ++ [x]) 
+  translatesTo remap_env frmap (Γ ++ [x]) b ann_b b' ->
+  translatesTo remap_env frmap (Γ ++ [x]) 
     (csubst v (List.length Γ) b) (annot_csubst ann_v (List.length Γ) ann_b) b'.
 Proof.
-  intros Σ_fresh Γ x b. revert Γ. induction b; 
+  intros frmap Γ x b. revert Γ. induction b; 
   intros Γ ann_b b' v ann_v Hin tlt; inversion tlt.
   - constructor.
   - simpl. unfold find_index_string in H1.
@@ -322,16 +292,16 @@ Proof.
   - now eapply tlt_const.
 Qed.
 
-Lemma csubst_correct : forall Σ_fresh Γ x v b ann_v ann_b v' b',
+Lemma csubst_correct : forall frmap Γ x v b ann_v ann_b v' b',
   ~ In x Γ ->
-  ~ In x (get_binder_names Σ_fresh) ->
-  translatesTo remap_env Σ_fresh [] v ann_v v' ->
-  translatesTo remap_env Σ_fresh (Γ ++ [x]) b ann_b b' ->
-  translatesTo remap_env Σ_fresh Γ (csubst v (List.length Γ) b)
+  ~ In x (get_binder_names frmap) ->
+  translatesTo remap_env frmap [] v ann_v v' ->
+  translatesTo remap_env frmap (Γ ++ [x]) b ann_b b' ->
+  translatesTo remap_env frmap Γ (csubst v (List.length Γ) b)
   (annot_csubst ann_v (List.length Γ) ann_b)
   (BigStepPIR.subst x v' b').
 Proof.
-  intros Σ_fresh Γ x v b. revert Γ. induction b;
+  intros frmap Γ x v b. revert Γ. induction b;
   intros Γ ann_v ann_b v' b' HnIn HnIn' tlt_v tlt_b;
   inversion tlt_b; subst.
   - constructor.
@@ -354,9 +324,9 @@ Proof.
     + apply tlt_lambda. 
       * assumption.
       * subst x'. assert (Hin : In x (x::Γ)) by now left.
-        specialize (csubst_shadowed Σ_fresh (x :: Γ) x b ann_b0 b'0 v ann_v Hin H4).
+        specialize (csubst_shadowed frmap (x :: Γ) x b ann_b0 b'0 v ann_v Hin H4).
         intros. simpl in H.
-        specialize (strengthen_shadowed_ctx Σ_fresh (x :: Γ) x 
+        specialize (strengthen_shadowed_ctx frmap (x :: Γ) x 
           (csubst v (S #|Γ|) b) (annot_csubst ann_v (S #|Γ|) ann_b0) b'0 Hin H) as Hctx'.
         apply Hctx'.
     + apply tlt_lambda.
@@ -368,9 +338,9 @@ Proof.
       * assumption.
       * now apply IHb1. 
       * subst x'. assert (Hin : In x (x::Γ)) by now left.
-        specialize (csubst_shadowed Σ_fresh (x :: Γ) x b2 ann_b0 b'0 v ann_v Hin H6).
+        specialize (csubst_shadowed frmap (x :: Γ) x b2 ann_b0 b'0 v ann_v Hin H6).
         intros. simpl in H.
-        specialize (strengthen_shadowed_ctx Σ_fresh (x :: Γ) x 
+        specialize (strengthen_shadowed_ctx frmap (x :: Γ) x 
           (csubst v (S #|Γ|) b2) (annot_csubst ann_v (S #|Γ|) ann_b0) b'0 Hin H) as Hctx'.
         apply Hctx'.
     + apply tlt_let.
@@ -411,7 +381,7 @@ Proof with (eauto using eval).
     inversion tlt_l. subst.
     assert (tlt_sb : translatesTo remap_env [] [] (csubst a' 0 b) (annot_csubst ann_v2 0 ann_b) (BigStepPIR.subst x' v2' b')).
     { eapply csubst_correct; auto. }
-    eapply tlt_in_sub in tlt_sb as sub_sb.
+    eapply (tlt_in_sub remap_env [] [] tt) in tlt_sb as sub_sb; try constructor.
     specialize (IHev3 (annot_csubst ann_v2 0 ann_b) sub_sb sub_v (subst x' v2' b') tlt_sb).
     destruct IHev3 as [ann_v' [v' [k3 [tlt_v ev_v]]]].
     exists ann_v'. exists v'. eexists. split.
@@ -427,7 +397,7 @@ Proof with (eauto using eval).
     destruct (IHev1 ann_br H1 sub_br br' H10) as [ann_v1 [v1' [k1 [tlt_br ev_br]]]].
     assert (tlt_sb : translatesTo remap_env [] [] (csubst b0' 0 b1) (annot_csubst ann_v1 0 ann_b) (BigStepPIR.subst x'0 v1' b')).
     { eapply csubst_correct; auto. }
-    eapply tlt_in_sub in tlt_sb as sub_sb.
+    eapply (tlt_in_sub remap_env [] [] tt) in tlt_sb as sub_sb; try constructor.
     specialize (IHev2 (annot_csubst ann_v1 0 ann_b) sub_sb sub_v (subst x'0 v1' b') tlt_sb).
     destruct IHev2 as [ann_v' [v' [k2 [tlt_v ev_v]]]].
     exists ann_v'. exists v'. eexists. split.
@@ -474,22 +444,24 @@ Proof with (eauto using eval).
     + apply E_LamAbs. eauto.
 Admitted.
 
-Theorem stlc_globals_correct : forall (Σ : global_env) ann_env Σ'
+(* globals and let binding the environment *)
+
+Theorem stlc_globals_correct : forall (eΣ : global_env) ann_env Σ'
   t (ann_t : annots box_type t) t' v,
-  (trans_env Σ) e⊢ t ⇓ v ->
-  EnvInSubset Σ ->
-  translate_env remap_env Σ ann_env = Ok Σ' ->
-  InSubset Σ [] t ->
-  translate_term remap_env (map fst Σ') [] t ann_t = Some t' ->
+  (trans_env eΣ) e⊢ t ⇓ v ->
+  EnvInSubset eΣ ->
+  translate_env remap_env eΣ ann_env = Ok Σ' ->
+  InSubset eΣ [] t ->
+  translate_term remap_env (to_fresh_map Σ') [] t ann_t = Some t' ->
   exists ann_v v' k,
-    translatesTo remap_env (map fst Σ') [] v ann_v v' /\
+    translatesTo remap_env (to_fresh_map Σ') [] v ann_v v' /\
     eval (subst_entries Σ' t') v' k.
 Proof with (eauto using eval).
-  intros Σ ann_env Σ' t ann_t t' v.
+  intros eΣ ann_env Σ' t ann_t t' v.
   intros ev sub_env tle sub_t tlt.
   apply translate_env_reflect in tle.
   apply translate_reflect in tlt; try apply NoDup_nil.
-  apply (val_in_sub Σ [] t v ev) in sub_t as sub_v.
+  apply (val_in_sub eΣ [] t v ev) in sub_t as sub_v.
   revert Σ' t' tle tlt; induction ev; 
   intros Σ' t'' tle tlt; inversion sub_t.
   - (* □ applied to values, temporary nonsensible case *) admit. 
@@ -500,10 +472,10 @@ Proof with (eauto using eval).
     destruct (IHev1 ann_t1 H1 sub_lambda Σ' t1' tle H5) as [ann_v1 [v1' [k1 [tlt_l ev_l]]]].
     destruct (IHev2 ann_t2 H2 sub_arg Σ' t2' tle H8) as [ann_v2 [v2' [k2 [tlt_v2 ev_v2]]]].
     inversion tlt_l. subst.
-    assert (tlt_sb : translatesTo remap_env (map fst Σ') [] 
+    assert (tlt_sb : translatesTo remap_env (to_fresh_map Σ') [] 
       (csubst a' 0 b) (annot_csubst ann_v2 0 ann_b) (BigStepPIR.subst x' v2' b')).
     { eapply csubst_correct; auto. simpl. admit. }
-    eapply tlt_in_sub in tlt_sb as sub_sb.
+    eapply (tlt_in_sub remap_env eΣ Σ' ann_env) in tlt_sb as sub_sb; try assumption.
     specialize (IHev3 (annot_csubst ann_v2 0 ann_b) sub_sb sub_v Σ' (BigStepPIR.subst x' v2' b') tle tlt_sb).
     destruct IHev3 as [ann_v' [v' [k3 [tlt_v ev_v]]]].
     exists ann_v'. exists v'. eexists. split.
@@ -517,17 +489,17 @@ Proof with (eauto using eval).
     inversion tlt. apply inj_pair2 in H8. subst.
     eapply val_in_sub in ev1 as sub_br; eauto.
     destruct (IHev1 ann_br H1 sub_br Σ' br' tle H10) as [ann_v1 [v1' [k1 [tlt_br ev_br]]]].
-    assert (tlt_sb : translatesTo remap_env (map fst Σ') [] 
+    assert (tlt_sb : translatesTo remap_env (to_fresh_map Σ') [] 
       (csubst b0' 0 b1) (annot_csubst ann_v1 0 ann_b) (BigStepPIR.subst x'0 v1' b')).
     { eapply csubst_correct; auto. admit. }
-    eapply tlt_in_sub in tlt_sb as sub_sb.
+    eapply (tlt_in_sub remap_env eΣ Σ' ann_env) in tlt_sb as sub_sb; try assumption.
     specialize (IHev2 (annot_csubst ann_v1 0 ann_b) sub_sb sub_v Σ' (subst x'0 v1' b') tle tlt_sb).
     destruct IHev2 as [ann_v' [v' [k2 [tlt_v ev_v]]]].
     exists ann_v'. exists v'. eexists. split.
     + apply tlt_v.
     + destruct Σ'.
       * simpl in *. econstructor. econstructor; simpl; eauto. 
-      * destruct e as [[e_kn e_kn'] [[vd ty] e_b']]. assert (e_kn' = vd) by admit. subst.
+      * destruct e as [e_kn [[vd ty] e_b']]. subst.
         erewrite unfold_let_subst_entries. simpl. admit.
   - (* mkApps fix *) 
     eapply val_in_sub in ev1 as sub_apps; eauto.
@@ -544,24 +516,13 @@ Proof with (eauto using eval).
     assert (decl = decl0 /\ body = cb) by eauto using declared_constant_same.
     invs H3. clear H0. clear H1.
     inversion tlt. subst.
-    destruct (lookup_init Σ Σ' ann_env c kn' decl0 cb isdecl e H1 tle) as [Σ'' [ann_cb [cb' tlt_cb]]].
+    destruct (lookup_init eΣ Σ' ann_env c kn' decl0 cb isdecl e H1 tle) as [Σ'' [ann_cb [cb' tlt_cb]]].
     (* declarations may be evaluated under a subset of the environment *)
-    assert (Σ'' = (map fst Σ')). { admit. } subst.
-    specialize (IHev ann_cb H2 sub_v Σ' cb' tle tlt_cb).
-    inversion tle; subst.
-    + discriminate.
-    + destruct decl; try inversion H3.
-      destruct entry as [[e_kn e_kn'] [[] e_b']].
-      destruct c0. destruct cst_body; simpl in H3; try eauto.
-      (* the names chosen for each entry is fresh *)
-      simpl. rewrite subst_entries_comm; [|admit].
-      simpl. destruct (b =? kn')%string.
-      * simpl in IHev. 
-          (* need to unfold subst_entries to the declaration *)
-          admit.
-      * (* this binder is not the one substituted for the variable *)
-          admit.
-    + (* type alias case *) admit.
+    assert (Σ'' = (to_fresh_map Σ')). { admit. } subst.
+    destruct (IHev ann_cb H2 sub_v Σ' cb' tle tlt_cb) as [ann_v' [v' [k [tl_v' ev_v']]]].
+    eexists. eexists. eexists. split.
+    + eapply tl_v'.
+    + (* will need to prove this under [Σ'1 ++ entry :: Σ'2] or by careful induction on the environment *) admit.
   - (* mkApps constr *)
     eapply val_in_sub in ev1 as sub_apps; eauto.
     apply mkApps_in_subset in sub_apps as [sub_constr _].
@@ -593,8 +554,6 @@ Proof with (eauto using eval).
     (* + apply E_LamAbs. eauto. *) 
 Admitted.
 
-(* globals and let binding the environment *)
-
 Theorem stlc_no_globals : forall
   t (ann_t : annots box_type t) t' v,
   [] e⊢ t ⇓ v ->
@@ -609,81 +568,54 @@ Proof with (eauto using eval).
   try discriminate; eauto. constructor.
 Qed.
 
-Theorem stlc_one_global : forall
-  gdecl (ann_env : env_annots box_type [gdecl]) entry t ann_t t' v,
-  (trans_env [gdecl]) e⊢ t ⇓ v ->
-  EnvInSubset [gdecl] ->
-  translate_env remap_env [gdecl] ann_env = Ok [entry] -> 
-  InSubset [gdecl] [] t ->
-  translate_term remap_env [fst entry] [] t ann_t = Some t' ->
-  exists ann_v v' k,
-    translatesTo remap_env [fst entry] [] v ann_v v' /\
-    eval (subst_entries [entry] t') v' k.
-Proof with (eauto using eval).
-  intros gdecl ann_env entry t ann_t t' v ev sub_env tle sub_t tlt.
-  apply translate_reflect in tlt; try apply NoDup_nil.
-  revert t' tlt; induction ev; 
-  intros t'' tlt; inversion sub_t.
-  - admit.
-  - destruct entry as [[e_kn e_kn'] [[vd ty'] b']]. subst.
-    admit.
-  - admit.
-  - subst. eapply val_in_sub, mkApps_in_subset in ev1 as [not_sub_fix _]; eauto.
-    inversion not_sub_fix.
-  - subst. eapply val_in_sub, mkApps_in_subset in ev1 as [not_sub_fix _]; eauto.
-    inversion not_sub_fix.
-  - admit.
-  - assert (decl = decl0 /\ body = cb) by eauto using declared_constant_same.
-    inversion tlt. invs H3. clear H0. clear H1.
-    destruct entry as [[e_kn e_kn'] [[vd ty] e_b']].
-    simpl. simpl in H6. admit.
+Lemma eval_let_subst_entries_equiv : forall Σ' t' v' k,
+  eval (subst_entries Σ' t') v' k ->
+  exists j, eval (Let (map snd Σ') t') v' j.
+Proof.
+  induction Σ'; intros.
+  - eauto.
+  - destruct a as [a_kn [[a_kn' a_ty'] a_b']].
+    simpl in *. rewrite subst_entries_comm in H; [|admit].
+    apply IHΣ' in H. destruct H. eexists.
+    constructor. econstructor; try eauto.
+    + admit.
+    + admit.
 Admitted.
 
-Lemma let_binding_env_correct : forall Σ' t ann_t t' t'',
-  translate_term remap_env (List.rev (map fst Σ')) [] t ann_t = Some t'' ->
-  translate_term remap_env [] [] t ann_t = Some (bind_pir_env Σ' t').
+Lemma eval_binding_subst_entries_equiv : forall Σ' t' v' k,
+  eval (subst_entries (List.rev Σ') t') v' k ->
+  exists j,
+    eval (bind_pir_env Σ' t') v' j.
 Proof.
-  intros. unfold bind_pir_env in *.
-  induction Σ'.
-Admitted.
-
-Lemma let_binding_eval_single : forall kn kn' ty br br' t' v' k i,
-  eval br br' k ->
-  eval (subst kn' br' t') v' i -> 
-  exists j, eval (bind_pir_env [((kn, kn'), TermBind (VarDecl kn' ty) br)] t') v' j.
-Proof.
-  intros. eexists.
-  unfold bind_pir_env. simpl.
-  constructor; eauto.
-  econstructor; eauto.
-  simpl. econstructor; eauto.
+  intros. unfold bind_pir_env in *. 
+  now eapply eval_let_subst_entries_equiv.
 Qed.
 
-Theorem stlc_program_correct : forall eΣ env_ann init cb t v t',
+Lemma let_binding_env_correct : forall eΣ Σ' t ann_t t' v ann_v v' j,
+  (trans_env eΣ) e⊢ t ⇓ v ->
+  translatesTo remap_env (to_fresh_map (List.rev Σ')) [] t ann_t t' /\
+  eval (subst_entries (List.rev Σ') t') v' j ->
+  exists (k : nat),
+    translatesTo remap_env [] [] v ann_v v' /\ 
+    eval (bind_pir_env Σ' t') v' k.
+Admitted.
+
+Theorem stlc_program_correct : forall eΣ ann_env init cb t v t',
   EGlobalEnv.declared_constant (trans_env eΣ) init cb ->
   cb.(cst_body) = Some t ->
   (trans_env eΣ) e⊢ t ⇓ v ->
   EnvInSubset eΣ ->
-  translate_typed_eprogram remap_env ((eΣ; env_ann), init) = Ok t' ->
+  translate_typed_eprogram remap_env ((eΣ; ann_env), init) = Ok t' ->
   exists ann_v v' k,
     translatesTo remap_env [] [] v ann_v v' /\
     eval t' v' k.
 Proof.
-  intros.
-  unfold translate_typed_eprogram in H3.
-  destruct (translate_env remap_env eΣ env_ann) as [Σ_fresh|] eqn:tle; try discriminate.
-  apply translate_env_reflect in tle.
-  destruct (lookup_entry Σ_fresh init) as [entry|] eqn:Hl; try discriminate.
-  induction tle; subst.
-  - inversion Hl.
-  - (* valid global *)
-    destruct decl; try inversion H4.
-    destruct entry0 as [[e_kn e_kn'] br].
-    destruct c. destruct br.
-    (* eapply (stlc_correct). *) admit.
-  - (* inductive is ignored instead of aborting the translation of the environment *)
-    hnf in H. simpl in H. 
-    destruct (init == kn); try discriminate.
-    unfold EGlobalEnv.declared_constant.
-    (* show that evaluation remains valid under the smaller environment *) admit.
+  intros. unfold translate_typed_eprogram in H3.
+  destruct (translate_env remap_env eΣ ann_env) as [Σ'|] eqn:tle; try discriminate.
+  destruct (lookup_entry Σ' init) as [entry|] eqn:Hl; try discriminate.
+  destruct entry as [e_kn [[vd ty'] b']]. inversion H3. subst.
+  evar (ann_t : annots box_type t). eexists ?[ann_v]. eexists ?[v'].
+  eapply let_binding_env_correct; try eauto.
+  specialize (stlc_globals_correct eΣ ann_env (List.rev Σ') t ann_t (bind_pir_env Σ' (Var vd)) v H1 H2).
+  (* translateEnv is reversed compared to the term *) admit.
 Admitted.
