theories/Entry.v
@@ -1,0 +1,104 @@
+From MetaCoq.Erasure Require Import EAstUtils.
+From MetaCoq.Utils Require Import MCList MCString MCPrelude utils.
+
+From VTL Require Import Env PIR Utils.
+
+From Coq Require Import String BinInt List.
+
+Import EAst ExAst.
+Import BasicAst Kernames ListNotations.
+Import MCMonadNotation.
+
+Definition fresh_pair := kername * binderName. 
+Definition fresh_map := list (kername * binderName).
+
+Definition entry := kername * binding.
+
+Definition to_fresh_pair entry : fresh_pair :=
+  match entry with
+  | (kn, TermBind (VarDecl kn' ty') b') => (kn, kn')
+  end.
+
+Definition to_fresh_map (Σ' : list entry) : fresh_map :=
+  map to_fresh_pair Σ'.
+
+Definition get_entry_body (e : entry) : PIR.term :=
+  match e with
+  | (_, TermBind (VarDecl _ _) t') => t' 
+  end.
+
+Definition get_entry_nm (e : entry) : binderName :=
+  match e with
+  | (_, TermBind (VarDecl nm _) _) => nm
+  end.
+
+Definition get_binder_names (frmap : fresh_map) : list string :=
+  map snd frmap.
+
+Definition lookup_entry (Σ' : list entry) (nm : kername) : option entry :=
+  find (fun '(kn, _) => eq_kername kn nm) Σ'.
+
+Definition lookup_fresh (Σ_fresh : list fresh_pair) (nm : kername) : option fresh_pair :=
+  find (fun '(kn, _) => eq_kername kn nm) Σ_fresh.
+
+Lemma lookup_entry_key : forall Σ' k k' bnd,
+  lookup_entry Σ' k = Some (k', bnd) ->
+  k = k'.
+Proof.
+  intros. induction Σ'.
+  - inversion H.
+  - inversion H. destruct a.
+    destruct (k0 == k) eqn:Heq.
+    + now apply ReflectEq.eqb_eq in Heq. 
+    + inversion H. now rewrite Heq in H2.
+Qed.
+
+Lemma lookup_fresh_key : forall frmap k k' kn',
+  lookup_fresh frmap k = Some (k', kn') ->
+  k = k'.
+Proof.
+  intros. induction frmap.
+  - inversion H.
+  - inversion H. destruct a.
+    destruct (k0 == k) eqn:Heq.
+    + now apply ReflectEq.eqb_eq in Heq. 
+    + inversion H. now rewrite Heq in H2.
+Qed.
+
+Lemma lookup_entry_to_lookup_fresh : forall Σ' kn kn' ty' b',
+  lookup_entry Σ' kn = Some (kn, TermBind (VarDecl kn' ty') b') ->
+  lookup_fresh (to_fresh_map Σ') kn = Some (kn, kn').
+Proof.
+  intros. induction Σ'.
+  - inversion H.
+  - destruct a as [a_kn [[a_kn' a_ty'] a_b']]. simpl in *.
+    destruct (a_kn == kn) eqn:Heq.
+    + now inversion H.
+    + now apply IHΣ'.
+Qed.
+
+Lemma lookup_entry_Some : forall Σ' kn kn' ty' b', 
+  lookup_entry Σ' kn = Some (kn, TermBind (VarDecl kn' ty') b') ->
+  In kn' (map (snd ∘ to_fresh_pair) Σ').
+Proof.
+  intros. induction Σ'.
+  - discriminate.
+  - destruct a as [a_kn [[a_kn' a_ty'] a_b']]. 
+    simpl. simpl in H.
+    destruct (a_kn == kn) eqn:Heq; inversion H; subst.
+    + now left.
+    + apply IHΣ' in H1. now right.
+Qed.
+
+Lemma lookup_fresh_Some : forall frmap kn kn', 
+  lookup_fresh frmap kn = Some (kn, kn') ->
+  In kn' (get_binder_names frmap).
+Proof.
+  intros. induction frmap.
+  - discriminate.
+  - destruct a as [a_kn a_kn'].
+    simpl. simpl in H. eauto.
+    destruct (a_kn == kn) eqn:Heq; inversion H; subst.
+    + now left.
+    + apply IHfrmap in H1. now right.
+Qed.
